src/AST/Translator.Common.dfy
@@ -1,11 +1,16 @@
 include "../Interop/CSharpDafnyASTModel.dfy"
 include "../Interop/CSharpDafnyInterop.dfy"
 include "../Utils/Library.dfy"
+include "Locations.dfy"
+include "Syntax.dfy"
+include "Translator.Location.dfy"
 
 module Bootstrap.AST.Translator.Common {
   import opened Utils.Lib.Datatypes
   import opened Interop.CSharpDafnyInterop
   import C = Interop.CSharpDafnyASTModel
+  import opened L = Location
+  import Syntax.Debug
 
   datatype TranslationError =
     | Invalid(msg: string)
@@ -22,4 +27,20 @@ module Bootstrap.AST.Translator.Common {
 
   type TranslationResult<+A> =
     Result<A, TranslationError>
+
+  function method TranslateUnsupported(o: object?, descr: string)
+    : (e: Debug.Unsupported)
+    reads *
+  {
+    var loc :=
+      if o is C.Statement then
+        var s := o as C.Statement; TranslateLocation(s.Tok)
+      else if o is C.Expression then
+        var e := o as C.Expression; TranslateLocation(e.tok)
+      else if o is C.UserDefinedType then
+        var udt := o as C.UserDefinedType; TranslateLocation(udt.tok)
+      else
+        Locations.Location.EMPTY();
+    Debug.Unsupported(TypeConv.AnyToString(o), descr, loc)
+  }
 }
